EvmYul/Yul/SizeLemmas.lean
@@ -15,6 +15,7 @@ variable {expr arg : Expr}
          {exprs args args' : List Expr}
          {stmts : List Stmt}
          {f : FunctionDefinition}
+         {fName : YulFunctionName}
          {prim : PrimOp}
          {α : Type}
          {xs ys : List α}
@@ -91,7 +92,7 @@ lemma Stmt.zero_lt_sizeOf_List : 0 < sizeOf stmts := by cases stmts <;> aesop
 lemma FunctionDefinition.zero_lt_sizeOf : 0 < sizeOf f := by cases f; aesop
 
 @[simp]
-lemma Expr.sizeOf_args_lt_sizeOf_Call : sizeOf args < sizeOf (Call f args) := by
+lemma Expr.sizeOf_args_lt_sizeOf_Call : sizeOf args < sizeOf (Call fName args) := by
   simp
 
 @[simp]
